code/experimental/P256/Hacl.Impl.P256.fsti
@@ -135,7 +135,8 @@ val norm: p: point -> resultPoint: point -> tempBuffer: lbuffer uint64 (size 88)
       let zD = fromDomain_ (point_z_as_nat h0 p) in 
 
       let (xN, yN, zN) = _norm (xD, yD, zD) in 
-      x3 == xN /\ y3 == yN /\ z3 == zN 
+      x3 == xN /\ y3 == yN /\ z3 == zN /\
+      z3 == 1 
    )   
   )
 
@@ -181,7 +182,7 @@ val isPointAtInfinity: p: point -> Stack bool
       let x = as_nat h0 (gsub p (size 0) (size 4)) in 
       let y = as_nat h0 (gsub p (size 4) (size 4)) in 
       let z = as_nat h0 (gsub p (size 8) (size 4)) in 
-      r == isPointAtInfinity (x, y, z)
+      r == Hacl.Spec.P256.isPointAtInfinity (x, y, z)
     )
   ) 
 
